

Date: / /

(a) Distributive Property (Discrete time) - Proof.

$$\text{To prove: } f[n] * (g[n] + h[n]) = (f[n] * g[n]) + (f[n] * h[n])$$

By the definition of convolution, we know:

$$f[n] * g[n] = \sum_k f[k] \cdot g[n-k]$$

Similarly:

$$\text{LHS} = \sum_k f[k] \cdot (g+h)[n-k]$$

$$= \sum_k f[k] \cdot (g[n-k] + h[n-k])$$

$$= \sum_k (f[k] \cdot g[n-k] + f[k] \cdot h[n-k])$$

Splitting the summation across the addition, we get.

$$\text{LHS} = \sum_k f[k] \cdot g[n-k] + \sum_k f[k] \cdot h[n-k]$$

Now, consider RHS.

$$\text{RHS} = (f[n] * g[n]) + (f[n] * h[n])$$

By definition of convolution:

$$\text{RHS} = \sum_k f[k] \cdot g[n-k] + \sum_k f[k] \cdot h[n-k]$$

Thus, because $\text{LHS} = \text{RHS}$, we have proved the Distributive Property (Discrete time) of the convolution operator.

Date: / /

Ans 1. (b) Associative Property (Continuous-Time) - Proof.

$$\text{To prove: } (f(t) * g(t)) * h(t) = f(t) * (g(t) * h(t))$$

Consider LHS:

By definition of convolution.

$$f(t) * g(t) = \int f(\tau_1) \cdot g(t - \tau_1) d\tau_1 \quad \dots \textcircled{1}$$

$$\text{Now: } (f(t) * g(t)) * h(t)$$

$$= \int_{-\infty}^{\infty} \left[\int_{-\infty}^{\infty} f(\tau_1) \cdot g(\tau_2 - \tau_1) d\tau_1 \right] h(t - \tau_2) d\tau_2$$

--- Reasoning : [Consider $u(t) = f(t) * g(t)$]
----- $\textcircled{2}$

Then convolute $u(t)$ & $h(t)$

This will give:

$$\int u(\tau_2) \cdot h(t - \tau_2) d\tau_2.$$

Then substitute u from $\textcircled{1}$ & $\textcircled{2}$.

$$= \int_{-\infty}^{\infty} \int_{-\infty}^{\infty} f(\tau_1) \cdot g(\tau_2 - \tau_1) \cdot h(t - \tau_2) d\tau_1 d\tau_2.$$

Consider RHS:

$$u(t) = g(t) * h(t) = \int_{-\infty}^{\infty} g(\tau_1) \cdot h(t - \tau_1) d\tau_1 \quad \text{--- (3)}$$

$$\therefore f(t) * u(t) = \int_{-\infty}^{\infty} f(\tau_2) \cdot u(t - \tau_2) d\tau_2$$

Substituting from (1), the value of $u(t - \tau_2)$.

$$\begin{aligned} \text{RHS} &= \int_{-\infty}^{\infty} f(\tau_2) \left[\int_{-\infty}^{\infty} g(\tau_1) \cdot h((t - \tau_2) - \tau_1) d\tau_1 \right] d\tau_2 \\ &= \int_{-\infty}^{\infty} \int_{-\infty}^{\infty} f(\tau_2) \cdot g(\tau_1) \cdot h(t - \tau_2 - \tau_1) d\tau_1 d\tau_2 \quad \text{--- (4)} \end{aligned}$$

Consider LHS again:

$$\text{LHS} = \int_{-\infty}^{\infty} \int_{-\infty}^{\infty} f(\tau_1) \cdot g(\tau_2 - \tau_1) \cdot h(t - \tau_2) d\tau_1 d\tau_2$$

$$\text{Let } u = \tau_2 - \tau_1 \text{ \& } v = \tau_1$$

$$\therefore \tau_1 = v$$

$$\& \tau_2 = u + v$$

$$\frac{\partial(\tau_1, \tau_2)}{\partial(u, v)} = \begin{bmatrix} \frac{\partial \tau_1}{\partial u} & \frac{\partial \tau_1}{\partial v} \\ \frac{\partial \tau_2}{\partial u} & \frac{\partial \tau_2}{\partial v} \end{bmatrix} = \begin{bmatrix} 0 & 1 \\ 1 & 1 \end{bmatrix}$$

$$|J| = 1$$

Date: / /

$$\therefore \text{LHS} = \int_{-\infty}^{\infty} \int_{-\infty}^{\infty} f(v) \cdot g(u) \cdot h(t-u-v) \, du \cdot dv.$$

Rename: $v = \tau_2$, $u = \tau_1$.

$$\text{We get LHS} = \int_{-\infty}^{\infty} \int_{-\infty}^{\infty} f(\tau_2) \cdot g(\tau_1) \cdot h(t-\tau_1-\tau_2) \, d\tau_1 \, d\tau_2$$

$\therefore \text{LHS} = \text{RHS}$.

Thus we have proved associative property of convolution in continuous time.